experiments/state_on_io/Free.fst
@@ -3,9 +3,9 @@ module Free
 (** Sum of two command types.
     Commands are indexed types (Type0 -> Type) parameterizing the free monad. *)
 noeq
-type cmd_sum (cmd1 cmd2 : Type0 -> Type) : Type0 -> Type =
-| CmdL : #r:Type0 -> cmd1 r -> cmd_sum cmd1 cmd2 r
-| CmdR : #r:Type0 -> cmd2 r -> cmd_sum cmd1 cmd2 r
+type cmd_sum (cmd1 cmd2 : Type -> Type) : Type -> Type =
+| CmdL : #r:Type -> cmd1 r -> cmd_sum cmd1 cmd2 r
+| CmdR : #r:Type -> cmd2 r -> cmd_sum cmd1 cmd2 r
 
 (** Sum of two event types.
     Events are plain types parameterizing the hist monad. *)
@@ -21,10 +21,11 @@ type free (cmd : Type u#i -> Type u#e) (a:Type u#a) : Type u#(max (1 + i) (max a
 | Call : caller -> #r:Type u#i -> cmd r -> cont:(r -> free cmd a) -> free cmd a
 | Return : a -> free cmd a
 
+val free_return : #cmd:(Type u#i -> Type u#e) -> #a:Type u#a -> x:a -> free cmd a
 let free_return #cmd #a (x:a) : free cmd a =
   Return x
 
-#set-options "--print_universes"
+val free_bind : #cmd:(Type u#i -> Type u#e) -> #a:Type u#a -> #b:Type u#b -> l:free cmd a -> k:(a -> free cmd b) -> free cmd b
 let rec free_bind
   #cmd #a #b
   (l : free cmd a)
@@ -36,6 +37,7 @@ let rec free_bind
       Call c op (fun i ->
         free_bind (fnc i) k)
 
+val free_map : #cmd:(Type u#i -> Type u#e) -> #a:Type u#a -> #b:Type u#b -> l:free cmd a -> k:(a -> b) -> Tot (free cmd b)
 let free_map
   #cmd #a #b
   (l : free cmd a)
